\documentclass[preview, convert={outfile=\jobname.svg}]{standalone}
\usepackage{amsmath}

\begin{document}
\begin{equation*}
    \begin{cases}
            l_1\ddot{\theta_1} + 2\dot{l_1}\dot{\theta_1} = -g\sin\theta_1 + r\dot{\theta_1}^2 \\
            l_2\ddot{\theta_2} + 2\dot{l_2}\dot{\theta_2} = -g\sin\theta_2 + r\dot{\theta_2}^2 \\
                (m_1 + m_2)\ddot{x} = -m_1g\cos\theta_1 + m_2g\cos\theta_2 - m_1l_1\dot{\theta_1}^2 + m_2l_2\dot{\theta_2}^2
    \end{cases}\!\!\!.
\end{equation*}
\end{document}